<?xml version="1.0" encoding="UTF-8"?>
<rdf:RDF
        xmlns:dc="http://purl.org/dc/terms/"
        xmlns:rdf="http://www.w3.org/1999/02/22-rdf-syntax-ns#"
        xmlns:skos="http://www.w3.org/2004/02/skos/core#"
        >
    <rdf:Description rdf:about="http://purl.org/anzsrc/toa/#strategic">
        <rdf:type rdf:resource="http://www.w3.org/2004/02/skos/core#Concept"/>
        <skos:prefLabel xml:lang="en">Strategic basic research</skos:prefLabel>
        <skos:inScheme rdf:resource="http://purl.org/anzsrc/toa/#toa"/>
        <skos:scopeNote xml:lang="en">Strategic basic research is experimental and theoretical work undertaken to
            acquire new knowledge directed into specified broad areas in the expectation of practical discoveries. It
            provides the broad base of knowledge necessary for the solution of recognised practical problems.
        </skos:scopeNote>
    </rdf:Description>
    <rdf:Description rdf:about="http://purl.org/anzsrc/toa/#applied">
        <rdf:type rdf:resource="http://www.w3.org/2004/02/skos/core#Concept"/>
        <skos:prefLabel xml:lang="en">Applied research</skos:prefLabel>
        <skos:inScheme rdf:resource="http://purl.org/anzsrc/toa/#toa"/>
        <skos:scopeNote xml:lang="en">Strategic basic research is experimental and theoretical work undertaken to
            acquire new knowledge directed into specified broad areas in the expectation of practical discoveries. It
            provides the broad base of knowledge necessary for the solution of recognised practical problems.
        </skos:scopeNote>
    </rdf:Description>
    <rdf:Description rdf:about="http://purl.org/anzsrc/toa/#experimental">
        <rdf:type rdf:resource="http://www.w3.org/2004/02/skos/core#Concept"/>
        <skos:prefLabel xml:lang="en">Experimental development</skos:prefLabel>
        <skos:inScheme rdf:resource="http://purl.org/anzsrc/toa/#toa"/>
        <skos:scopeNote xml:lang="en">Strategic basic research is experimental and theoretical work undertaken to
            acquire new knowledge directed into specified broad areas in the expectation of practical discoveries. It
            provides the broad base of knowledge necessary for the solution of recognised practical problems.
        </skos:scopeNote>
    </rdf:Description>
    <rdf:Description rdf:about="http://purl.org/anzsrc/toa/#basic">
        <rdf:type rdf:resource="http://www.w3.org/2004/02/skos/core#Concept"/>
        <skos:prefLabel xml:lang="en">Pure basic research</skos:prefLabel>
        <skos:inScheme rdf:resource="http://purl.org/anzsrc/toa/#toa"/>
        <skos:scopeNote xml:lang="en">Pure basic research is experimental and theoretical work undertaken to acquire new
            knowledge without looking for long term benefits other than the advancement of knowledge.
        </skos:scopeNote>
    </rdf:Description>
</rdf:RDF>
